src/QueryStructure/Implementation/Operations/BagADT/Refinements.v
@@ -77,6 +77,23 @@ Section BagsQueryStructureRefinements.
     intros; simpl; rewrite i2th_replace_BoundIndex_neq; eauto using string_dec.
   Qed.
 
+  (* Cross product of lists using heterogenous lists. *)
+    Definition Join_Lists
+             {A : Type}
+             {f : A -> Type}
+             {As : list A}
+             {a : A}
+             (l : list (f a))
+             (l' : list (ilist f As))
+  : list (ilist f (a :: As)) :=
+    (flat_map (fun l' => map (fun fa => icons _ fa l') l) l').
+
+  Definition Build_single_Tuple_list
+             {heading}
+             (l : list (@Tuple heading))
+  : list (ilist (@Tuple) [heading])
+    := map (fun a => icons _ a (inil _)) l.
+
   Lemma refine_Query_In_Enumerate
         (ResultT : Type) :
     forall r_o (r_n : IndexedQueryStructure qs_schema BagIndexKeys),
@@ -85,7 +102,8 @@ Section BagsQueryStructureRefinements.
                 (resultComp : Tuple -> Comp (list ResultT)),
            refine (UnConstrQuery_In r_o idx resultComp)
                   (l <- CallBagMethod idx {|bindex := "Enumerate" |} r_n ();
-                   List_Query_In (snd l) resultComp).
+                   List_Query_In (Build_single_Tuple_list (snd l))
+                                 (fun tup => resultComp (ilist_hd tup))) .
   Proof.
     unfold UnConstrQuery_In, QueryResultComp, CallBagMethod;
     intros; simpl.
@@ -98,6 +116,28 @@ Section BagsQueryStructureRefinements.
     intuition; destruct_ex; intuition; subst.
     econstructor; eauto.
     econstructor; rewrite (H idx); eauto.
+    unfold Build_single_Tuple_list in *; rewrite map_map.
+    repeat rewrite map_map in H2; simpl in *; eauto.
+  Qed.
+
+  Local Transparent Query_For.
+
+  Lemma refine_For_Enumerate
+        (ResultT : Type) :
+    forall r_o (r_n : IndexedQueryStructure qs_schema BagIndexKeys),
+      DelegateToBag_AbsR r_o r_n
+      -> forall (idx : BoundedString)
+                (f : _ -> Comp (list ResultT)),
+           refine (For (l <- CallBagMethod idx {|bindex := "Enumerate" |} r_n ();
+                        f l))
+                  (l <- CallBagMethod idx {|bindex := "Enumerate" |} r_n ();
+                   For (f l)).
+  Proof.
+    simpl; intros; unfold Query_For.
+    simplify with monad laws.
+    unfold CallBagMethod; simpl.
+    unfold refine; intros; inversion_by computes_to_inv.
+    subst; econstructor; econstructor; eauto.
   Qed.
 
   Lemma flatten_CompList_app_inv
@@ -118,23 +158,26 @@ Section BagsQueryStructureRefinements.
       repeat econstructor; eauto.
   Qed.
 
+
   Lemma refine_Join_Query_In_Enumerate'
-        heading
+        headings
         (ResultT : Type) :
     forall r_o (r_n : IndexedQueryStructure qs_schema BagIndexKeys),
       DelegateToBag_AbsR r_o r_n ->
       forall (idx : BoundedString)
-             (resultComp : Tuple -> Tuple -> Comp (list ResultT))
+             (resultComp : ilist (@Tuple) headings
+                           -> Tuple
+                           -> Comp (list ResultT))
              l,
-        refine (List_Query_In l (fun tup : @Tuple heading =>
+        refine (List_Query_In l (fun tup : ilist (@Tuple) headings =>
                                    UnConstrQuery_In r_o idx (resultComp tup)))
                (l' <- CallBagMethod idx {|bindex := "Enumerate" |} r_n ();
-                List_Query_In (Join_Lists l (snd l'))
-                              (fun tup_pair => (resultComp (fst tup_pair) (snd tup_pair)))).
+                List_Query_In (Join_Lists (snd l') l)
+                              (fun tup_pair => (resultComp (ilist_tl tup_pair) (ilist_hd tup_pair)))).
   Proof.
     intros.
     unfold List_Query_In; induction l; simpl.
-    - intros v Comp_v; inversion_by computes_to_inv; subst; constructor.
+    - intros v Comp_v; inversion_by computes_to_inv; subst; eauto.
     - setoid_rewrite IHl; rewrite refine_Query_In_Enumerate; eauto.
       unfold List_Query_In.
       setoid_rewrite refineEquiv_bind_bind at 1.
@@ -144,6 +187,8 @@ Section BagsQueryStructureRefinements.
       econstructor; eauto.
       apply flatten_CompList_app_inv in H2; destruct_ex; intuition.
       subst; repeat (econstructor; eauto).
+      unfold Build_single_Tuple_list in *; rewrite map_map; simpl;
+      eauto.
   Qed.
 
   Corollary refine_Join_Query_In_Enumerate
@@ -153,16 +198,17 @@ Section BagsQueryStructureRefinements.
       forall (idx idx' : BoundedString)
              (resultComp : Tuple -> Tuple -> Comp (list ResultT)),
         refine (l <- CallBagMethod idx {|bindex := "Enumerate" |} r_n ();
-                List_Query_In (snd l) (fun tup : Tuple =>
-                                          UnConstrQuery_In r_o idx' (resultComp tup)))
+                List_Query_In (Build_single_Tuple_list (snd l))
+                              (fun tup =>
+                                 UnConstrQuery_In r_o idx' (resultComp (ilist_hd tup))))
                (l <- CallBagMethod idx {|bindex := "Enumerate" |} r_n ();
                 l' <- CallBagMethod idx' {|bindex := "Enumerate" |} r_n ();
-                List_Query_In (Join_Lists (snd l) (snd l'))
-                              (fun tup_pair => (resultComp (fst tup_pair) (snd tup_pair)))).
+                List_Query_In (Join_Lists (snd l') (Build_single_Tuple_list (snd l)))
+                              (fun tup_pair => (resultComp (ilist_hd (ilist_tl tup_pair)) (ilist_hd tup_pair)))).
   Proof.
     intros.
     f_equiv; simpl; intro.
-    apply refine_Join_Query_In_Enumerate'; eauto.
+    eapply refine_Join_Query_In_Enumerate'; eauto.
   Qed.
 
   Lemma refine_Join_Enumerate_Swap
@@ -180,8 +226,6 @@ Section BagsQueryStructureRefinements.
     inversion_by computes_to_inv; subst;
     repeat (econstructor; eauto).
   Qed.
-
-  Local Transparent Query_For.
 
   Lemma refine_Query_For_In_Find
         (ResultT : Type)
@@ -209,24 +253,125 @@ Section BagsQueryStructureRefinements.
     intros v Comp_v; econstructor; eauto.
   Qed.
 
-  Instance DecideableEnsemblePair_snd {A B}
-           (P : Ensemble B) 
+  Instance DecideableEnsemblePair_tail
+           {A}
+           {a}
+           {As}
+           (f : A -> Type)
+           (P : Ensemble (ilist f As))
            (P_dec : DecideableEnsemble P)
-  : DecideableEnsemble (fun ab : A * B => P (snd ab)) :=
-    {| dec ab := dec (snd ab) |}.
+  : DecideableEnsemble (fun ab : ilist f (a :: As) => P (ilist_tl ab)) :=
+    {| dec ab := dec (ilist_tl ab) |}.
   Proof.
-    destruct a; simpl; eapply dec_decides_P.
+    intro; apply (dec_decides_P (DecideableEnsemble := P_dec) (ilist_tl a0)).
   Defined.
 
-  Instance DecideableEnsemblePair_fst {A B}
-           (P : Ensemble A) 
+  Instance DecideableEnsemblePair_head
+           {A}
+           {a}
+           {As}
+           (f : A -> Type)
+           (P : Ensemble (f a))
            (P_dec : DecideableEnsemble P)
-  : DecideableEnsemble (fun ab : A * B => P (fst ab)) :=
-    {| dec ab := dec (fst ab) |}.
+  : DecideableEnsemble (fun ab : ilist f (a :: As) => P (ilist_hd ab)) :=
+    {| dec ab := dec (ilist_hd ab) |}.
   Proof.
-    destruct a; simpl; eapply dec_decides_P.
+    intro; apply (dec_decides_P (DecideableEnsemble := P_dec) (ilist_hd a0)).
   Defined.
-  
+
+  Lemma filter_join_ilist_hd
+        {A}
+        {a}
+        {As}
+        (f' : A -> Type)
+  : forall
+      (f : f' a -> bool)
+      (s2 : list (ilist f' As))
+      (s1 : list (f' a)),
+      filter (fun x : ilist f' (a :: As) => f (ilist_hd x))
+             (Join_Lists s1 s2) =
+      Join_Lists (filter f s1) s2.
+  Proof.
+    induction s2; simpl; intros; eauto.
+    rewrite filter_app, IHs2; f_equal.
+    induction s1; simpl; eauto.
+    rewrite IHs1; destruct (f a1); simpl; eauto.
+  Qed.
+
+  Lemma Join_Lists_nil
+        {A}
+        {a}
+        {As}
+        (f' : A -> Type)
+  : forall (s2 : list (ilist f' As)),
+      Join_Lists (a := a) [] s2 = [].
+  Proof.
+    induction s2; simpl; eauto.
+  Qed.
+
+  Lemma filter_join_ilist_tail
+        {A}
+        {a}
+        {As}
+        (f' : A -> Type)
+  : forall
+      (f : (ilist f' As) -> bool)
+      (s2 : list (ilist f' As))
+      (s1 : list (f' a)),
+      filter (fun x : ilist f' (a :: As) => f (ilist_tl x))
+                (Join_Lists s1 s2) =
+      Join_Lists s1 (filter f s2).
+  Proof.
+    induction s2; simpl; intros; eauto.
+    rewrite filter_app, IHs2.
+    rewrite filter_map; simpl.
+    induction s1; simpl.
+    - repeat rewrite Join_Lists_nil; eauto.
+    - destruct (f a0); simpl; eauto.
+      + f_equal; simpl in *.
+        rewrite filter_true; reflexivity.
+      + rewrite filter_false in *; reflexivity.
+  Qed.
+
+  Lemma filter_Build_single_Tuple_list
+        {heading}
+        (l : list (@Tuple heading))
+        (filter_dec : @Tuple heading -> bool)
+  : filter (fun tup : ilist (@Tuple) [_] => filter_dec (ilist_hd tup)) (Build_single_Tuple_list l) = Build_single_Tuple_list (filter filter_dec l).
+  Proof.
+    induction l; simpl; eauto.
+    destruct (filter_dec a); simpl; congruence.
+  Qed.
+
+  Corollary refine_Query_For_In_Find'
+        (ResultT : Type)
+  : forall r_o (r_n : IndexedQueryStructure qs_schema BagIndexKeys),
+      DelegateToBag_AbsR r_o r_n
+      ->
+      forall (idx : @BoundedString (map relName (qschemaSchemas qs_schema)))
+             (filter_dec : Tuple -> bool)
+             search_pattern
+             (resultComp : _ -> Comp (list ResultT)),
+        ExtensionalEq filter_dec
+                      (BagMatchSearchTerm (ith_Bounded relName BagIndexKeys idx) search_pattern)
+        -> refine (For (l <- CallBagMethod idx {|bindex := "Enumerate" |} r_n ();
+                        List_Query_In (filter (fun tup : ilist (@Tuple) [_] => filter_dec (ilist_hd tup)) (Build_single_Tuple_list (snd l)))
+                                      resultComp))
+                  (l <- CallBagMethod idx {|bindex := "Find" |} r_n search_pattern;
+                   List_Query_In (Build_single_Tuple_list (snd l)) resultComp).
+  Proof.
+    simpl; intros.
+    setoid_rewrite filter_Build_single_Tuple_list.
+    unfold UnConstrQuery_In, QueryResultComp, CallBagMethod, Query_For;
+    intros; simpl.
+    simplify with monad laws.
+    setoid_rewrite refineEquiv_bind_bind;
+      setoid_rewrite refineEquiv_bind_unit; simpl; f_equiv; intro.
+    unfold List_Query_In.
+    rewrite (filter_by_equiv _ _ H0).
+    intros v Comp_v; econstructor; eauto.
+  Qed.
+
   Lemma refine_Join_Lists_Where_snd
         (ResultT : Type) :
     forall (r_n : IndexedQueryStructure qs_schema BagIndexKeys) idx idx'
@@ -238,35 +383,39 @@ Section BagsQueryStructureRefinements.
                     (BagMatchSearchTerm (ith_Bounded relName BagIndexKeys idx') search_pattern)
       -> refine (For (l <- CallBagMethod idx {| bindex := "Enumerate" |} r_n ();
                       l' <- CallBagMethod idx' {| bindex := "Enumerate" |} r_n ();
-                      List_Query_In (Join_Lists (snd l) (snd l'))
-                                    (fun tup_pair : Tuple * Tuple =>
-                                       Where (DT (snd tup_pair))
-                                             (resultComp (fst tup_pair) (snd tup_pair)))))
+                      List_Query_In (Join_Lists (snd l') (Build_single_Tuple_list (snd l)))
+                                    (fun tup_pair =>
+                                       Where (DT (ilist_hd tup_pair))
+                                             (resultComp (ilist_hd tup_pair) (ilist_hd (ilist_tl tup_pair))))))
 
                 (For (l <- CallBagMethod idx {| bindex := "Enumerate" |} r_n ();
                       l' <- CallBagMethod idx' {| bindex := "Find" |} r_n search_pattern;
-                      List_Query_In (Join_Lists (snd l) (snd l'))
-                                    (fun tup_pair : Tuple * Tuple =>
-                                       (resultComp (fst tup_pair) (snd tup_pair))))).
+                      List_Query_In
+                        (Join_Lists (snd l') (Build_single_Tuple_list (snd l)))
+                                    (fun tup_pair =>
+                                       (resultComp (ilist_hd tup_pair) (ilist_hd (ilist_tl tup_pair)))))).
   Proof.
     intros; repeat f_equiv; simpl; intro.
     unfold CallBagMethod; simpl.
     repeat setoid_rewrite refineEquiv_bind_bind;
-      repeat setoid_rewrite refineEquiv_bind_unit; 
+      repeat setoid_rewrite refineEquiv_bind_unit;
       f_equiv; unfold pointwise_relation; intro; simpl.
     setoid_rewrite <- (filter_by_equiv _ _ H).
     setoid_rewrite refine_List_Query_In_Where; simpl.
-    rewrite <- filter_join_snd; f_equiv.
+    instantiate (1 := _); simpl.
+    rewrite filter_join_ilist_hd; f_equiv.
   Qed.
-    
+
   Lemma refine_List_Query_In_Return
-        (ResultT : Type) :
-    forall l,
-      refine (List_Query_In l (@Query_Return ResultT) ) (ret l).
+        (ElementT ResultT : Type):
+    forall (l : list ElementT)
+           (f : ElementT -> ResultT),
+      refine (List_Query_In l (fun el => Query_Return (f el)) ) (ret (map f l)).
   Proof.
-    unfold List_Query_In; induction l; simpl.
+    unfold List_Query_In; induction l; intros; simpl.
     - reflexivity.
-    - simplify with monad laws; rewrite IHl; simplify with monad laws;
+    - unfold Query_Return; simplify with monad laws;
+      setoid_rewrite IHl; simplify with monad laws;
       reflexivity.
   Qed.
 
@@ -289,8 +438,12 @@ Section BagsQueryStructureRefinements.
     intros; setoid_rewrite DeletedTuplesFor; auto.
     rewrite refine_Query_In_Enumerate by eauto.
     setoid_rewrite refine_List_Query_In_Where.
-    rewrite (refine_Query_For_In_Find H Query_Return H0).
+    instantiate (1 := _).
+    simpl in *.
+    setoid_rewrite (refine_Query_For_In_Find' H _ H0).
     setoid_rewrite refine_List_Query_In_Return.
+    unfold Build_single_Tuple_list; setoid_rewrite map_map; simpl.
+    setoid_rewrite map_id.
     unfold CallBagMethod; simpl; simplify with monad laws;
     setoid_rewrite refineEquiv_bind_bind;
     setoid_rewrite refineEquiv_bind_unit; simpl;
